\documentclass{ximera}

\input{../../../preamble.tex}
\author{Chris Black}
\license{GFDL}

\begin{document}

\begin{exercise}
  Assume
  \[
    \alpha\colvector{3\\2\\-2}+
    \colvector{6\\1\\2}
    =
    \colvector{0\\-3\\6}.
  \]

  \begin{hint}
    Performing the indicated operations, we obtain the vector equations
    \begin{align*}
      \colvector{3\alpha \\ 2\alpha\\ - 2\alpha} + \colvector{6\\1\\2}
   &= \colvector{3\alpha + 6 \\ 2\alpha + 1\\ -2\alpha + 2}
      = \colvector{0\\-3\\6}
    \end{align*}
  \end{hint}

  \begin{hint}
    Thus, if a solution $\alpha$ exists then $\alpha$ must satisfy the three equations:
    \begin{align*}
      3\alpha + 6 &= 0\\
      2\alpha + 1 &= -3\\
      -2 \alpha + 2 &= 6
    \end{align*}
  \end{hint}

  \begin{hint}
    This leads to $3\alpha = -6$, $2\alpha = -4$ and $-2\alpha = 4$.
  \end{hint}
  
  \begin{hint}  
    And thus, the solution to the given vector equation is $\alpha = -2$.
  \end{hint}

  Then $\alpha = \answer{-2}$.

\end{exercise}

\end{document}

